rupicola/io/STLC.fst
@@ -742,7 +742,7 @@ let indexed_sem_expr_shape (t:typ) (e:closed_exp) (h:history) : Tot Type0 =
 let lem_value_preserves_value (e:closed_exp) (h:history) (t:typ) :
   Lemma (requires is_value e /\ sem_value_shape t e)
         (ensures indexed_sem_expr_shape t e h) =
-  introduce forall e' lt. steps e e' h lt /\ indexed_irred e' (h++lt) ==> sem_value_shape t e' with begin 
+  introduce forall e' lt. steps e e' h lt /\ indexed_irred e' (h++lt) ==> sem_value_shape t e' with begin
     introduce _ ==> _ with _. begin
       lem_value_is_irred e;
       FStar.Squash.bind_squash #(steps e e' h lt) () (fun sts ->
@@ -940,6 +940,7 @@ let can_step_eif_when_safe (e1 e2 e3:closed_exp) (h:history) : Lemma
     end
   end
 
+#push-options "--split_queries always"
 let rec destruct_steps_eif
   (e1:closed_exp)
   (e2:closed_exp)
@@ -948,16 +949,18 @@ let rec destruct_steps_eif
   (h:history)
   (lt:local_trace h)
   (st:steps (EIf e1 e2 e3) e' h lt) :
-  Pure (closed_exp * (lt1:local_trace h & (local_trace (h++lt1) * local_trace (h++lt1))))
+  Pure (closed_exp * (lt1:local_trace h & local_trace (h++lt1)))
     (requires indexed_irred e' (h++lt) /\
       indexed_sem_expr_shape TBool e1 h)
-    (ensures fun (e1', (| lt1, (lt2, lt3) |)) ->
+    (ensures fun (e1', (| lt1, lt2 |)) ->
       indexed_irred e1' (h++lt1) /\
+      is_value e1' /\
       steps e1 e1' h lt1 /\
       steps (EIf e1 e2 e3) (EIf e1' e2 e3) h lt1 /\
-      (ETrue? e1' ==> (steps e2 e' (h++lt1) lt2 /\ lt == lt1 @ lt2)) /\
-      (EFalse? e1' ==> (steps e3 e' (h++lt1) lt3 /\ lt == lt1 @ lt3)) /\
-      ((lt == lt1 @ lt2) \/ (lt == lt1 @ lt3)) /\
+      steps (EIf e1' e2 e3) e' (h++lt1) lt2 /\
+      (ETrue? e1' ==> (steps e2 e' (h++lt1) lt2)) /\
+      (EFalse? e1' ==> (steps e3 e' (h++lt1) lt2)) /\
+      (lt == lt1 @ lt2) /\
       (indexed_irred e1 h ==> (lt1 == [] /\ e1 == e1')))
     (decreases st)
   = match st with
@@ -975,22 +978,23 @@ let rec destruct_steps_eif
         let lt1 : local_trace h = as_lt oev1 in
         lem_step_preserve_indexed_sem_expr_shape e1 e1' h oev1 TBool;
         let s2 : steps (EIf e1' e2 e3) e' (h++lt1) lt23 = step_eif_steps in
-        let (e1'', (| lt1', (lt2, lt3) |)) = destruct_steps_eif e1' e2 e3 e' (h++lt1) lt23 s2 in
+        let (e1'', (| lt1', lt2 |)) = destruct_steps_eif e1' e2 e3 e' (h++lt1) lt23 s2 in
         lem_steps_transitive e1 e1' e1'' h lt1 lt1';
         lem_steps_transitive (EIf e1 e2 e3) (EIf e1' e2 e3) (EIf e1'' e2 e3) h lt1 lt1';
-        (e1'', (| (lt1 @ lt1'), (lt2, lt3) |))
+        (e1'', (| (lt1 @ lt1'), lt2 |))
         end
       | IfTrue e2 e3 h -> begin
         lem_step_implies_steps (EIf e1 e2 e3) e2 h None;
         lem_value_is_irred e1;
-        (e1, (| [], (lt, []) |))
+        (e1, (| [], lt |))
         end
       | IfFalse e2 e3 h -> begin
         lem_step_implies_steps (EIf e1 e2 e3) e3 h None;
         lem_value_is_irred e1;
-        (e1, (| [], ([], lt) |))
+        (e1, (| [], lt |))
         end
       end
+#pop-options
 
   (**
     How the steps look like:
@@ -1136,7 +1140,7 @@ let rec destruct_steps_epair_fst
   (e':closed_exp)
   (h:history)
   (lt:local_trace h)
-  (st:steps (EFst e12) e' h lt) 
+  (st:steps (EFst e12) e' h lt)
   (t1 t2:typ) :
   Pure (value * (lt12:local_trace h & local_trace (h++lt12)))
     (requires indexed_irred e' (h++lt) /\
@@ -1212,7 +1216,7 @@ let rec destruct_steps_epair_snd
   (e':closed_exp)
   (h:history)
   (lt:local_trace h)
-  (st:steps (ESnd e12) e' h lt) 
+  (st:steps (ESnd e12) e' h lt)
   (t1 t2:typ) :
   Pure (value * (lt12:local_trace h & local_trace (h++lt12)))
     (requires indexed_irred e' (h++lt) /\
@@ -1448,7 +1452,7 @@ let rec destruct_steps_ecase
   (e':closed_exp)
   (h:history)
   (lt:local_trace h)
-  (st:steps (ECase e_case e_lc e_rc) e' h lt) 
+  (st:steps (ECase e_case e_lc e_rc) e' h lt)
   (t1 t2:typ) :
   Pure (closed_exp * (lt1:local_trace h & (local_trace (h++lt1) * local_trace (h++lt1))))
     (requires indexed_irred e' (h++lt) /\
@@ -1513,7 +1517,7 @@ let rec destruct_steps_ecase
 #pop-options
 
 let can_step_eread_fd (fd:closed_exp{EFileDescr? fd}) (h:history) :
-  Lemma (exists e' oev. step (ERead fd) e' h oev) 
+  Lemma (exists e' oev. step (ERead fd) e' h oev)
   =
   let st1 : step (ERead fd) (EInl ETrue) h (Some (EvRead (get_fd fd) (Inl true))) = SReadReturn h (get_fd fd) (Inl true) in
     let st2 : step (ERead fd) (EInl EFalse) h (Some (EvRead (get_fd fd) (Inl false))) = SReadReturn h (get_fd fd) (Inl false) in
@@ -1522,7 +1526,7 @@ let can_step_eread_fd (fd:closed_exp{EFileDescr? fd}) (h:history) :
 
 let can_step_eread (fd:closed_exp) (h:history) :
   Lemma
-  (requires indexed_sem_expr_shape TFileDescr fd h)  
+  (requires indexed_sem_expr_shape TFileDescr fd h)
   (ensures (exists e' oev. step (ERead fd) e' h oev))
   =
   introduce indexed_irred fd h ==> (exists e' oev. step (ERead fd) e' h oev) with _. begin
@@ -1816,7 +1820,7 @@ let can_step_eopen_str (str:closed_exp{ETrue? str \/ EFalse? str}) (h:history) :
 
 let can_step_eopen (str:closed_exp) (h:history) :
   Lemma
-  (requires indexed_sem_expr_shape TBool str h)  
+  (requires indexed_sem_expr_shape TBool str h)
   (ensures (exists e' oev. step (EOpen str) e' h oev))
   =
   introduce indexed_irred str h ==> (exists e' oev. step (EOpen str) e' h oev) with _. begin
@@ -1921,7 +1925,7 @@ let destruct_steps_eopen
 
 let can_step_eclose (fd:closed_exp) (h:history) :
   Lemma
-  (requires indexed_sem_expr_shape TFileDescr fd h)  
+  (requires indexed_sem_expr_shape TFileDescr fd h)
   (ensures (exists e' oev. step (EClose fd) e' h oev))
   =
   introduce indexed_irred fd h ==> (exists e' oev. step (EClose fd) e' h oev) with _. begin
